<?xml version="1.0"?>


<!DOCTYPE rdf:RDF [
    <!ENTITY schema "http://schema.org/" >
    <!ENTITY org "http://www.w3.org/ns/org#" >
    <!ENTITY dcterms "http://purl.org/dc/terms/" >
    <!ENTITY foaf "http://xmlns.com/foaf/0.1/" >
    <!ENTITY vann "http://purl.org/vocab/vann/" >
    <!ENTITY owl "http://www.w3.org/2002/07/owl#" >
    <!ENTITY v1 "http://www.loc.gov/mads/rdf/v1#" >
    <!ENTITY v12 "http://purl.org/goodrelations/v1#" >
    <!ENTITY xsd "http://www.w3.org/2001/XMLSchema#" >
    <!ENTITY skos "http://www.w3.org/2004/02/skos/core#" >
    <!ENTITY rdfs "http://www.w3.org/2000/01/rdf-schema#" >
    <!ENTITY rdf "http://www.w3.org/1999/02/22-rdf-syntax-ns#" >
    <!ENTITY ns "http://www.w3.org/2003/06/sw-vocab-status/ns#" >
]>


<rdf:RDF xmlns="http://minetur.linkeddata.es/def/ontologiaProductos#"
     xml:base="http://minetur.linkeddata.es/def/ontologiaProductos"
     xmlns:v1="http://www.loc.gov/mads/rdf/v1#"
     xmlns:ns="http://www.w3.org/2003/06/sw-vocab-status/ns#"
     xmlns:foaf="http://xmlns.com/foaf/0.1/"
     xmlns:vann="http://purl.org/vocab/vann/"
     xmlns:org="http://www.w3.org/ns/org#"
     xmlns:dcterms="http://purl.org/dc/terms/"
     xmlns:schema="http://schema.org/"
     xmlns:rdfs="http://www.w3.org/2000/01/rdf-schema#"
     xmlns:xsd="http://www.w3.org/2001/XMLSchema#"
     xmlns:owl="http://www.w3.org/2002/07/owl#"
     xmlns:v12="http://purl.org/goodrelations/v1#"
     xmlns:rdf="http://www.w3.org/1999/02/22-rdf-syntax-ns#"
     xmlns:skos="http://www.w3.org/2004/02/skos/core#">
    <owl:Ontology rdf:about="http://minetur.linkeddata.es/def/ontologiaProductos#">
        <rdfs:label xml:lang="es">Ontología de productos para proyecto eoi (Escuela de Organización Industrial)</rdfs:label>
        <dcterms:created rdf:datatype="&xsd;date">2014-06-15</dcterms:created>
        <vann:preferredNamespaceUri rdf:datatype="&xsd;anyURI">http://minetur.linkeddata.es/def/ontologiaProductos#</vann:preferredNamespaceUri>
        <dcterms:license rdf:datatype="&xsd;anyURI">http://purl.oclc.org/NET/rdflicenses/allrightsreserved</dcterms:license>
        <dcterms:creator rdf:datatype="&xsd;anyURI">http://purl.org/net/mpoveda</dcterms:creator>
        <owl:versionInfo>1.0</owl:versionInfo>
        <dcterms:description xml:lang="es">Esta ontología para representar productos, empresas y clasificaciones de los mismos ha sido desarrollada por el Ontology Engineering Group en el contexto del proyecto piloto de desarrollo de ontologías para la Escuela de Organización Industrial.</dcterms:description>
        <dcterms:title xml:lang="es">Ontología de productos para proyecto eoi (Escuela de Organización Industrial)</dcterms:title>
        <vann:preferredNamespacePrefix>minetur</vann:preferredNamespacePrefix>
        <owl:imports rdf:resource="http://www.w3.org/2004/02/skos/core"/>
    </owl:Ontology>
    


    <!-- 
    ///////////////////////////////////////////////////////////////////////////////////////
    //
    // Annotation properties
    //
    ///////////////////////////////////////////////////////////////////////////////////////
     -->

    <owl:AnnotationProperty rdf:about="&ns;term_status"/>
    


    <!-- 
    ///////////////////////////////////////////////////////////////////////////////////////
    //
    // Datatypes
    //
    ///////////////////////////////////////////////////////////////////////////////////////
     -->

    


    <!-- 
    ///////////////////////////////////////////////////////////////////////////////////////
    //
    // Object Properties
    //
    ///////////////////////////////////////////////////////////////////////////////////////
     -->

    


    <!-- http://minetur.linkeddata.es/def/ontologiaProductos#esConsultorDe -->

    <owl:ObjectProperty rdf:about="http://minetur.linkeddata.es/def/ontologiaProductos#esConsultorDe">
        <rdfs:label xml:lang="es">es consultor de</rdfs:label>
        <rdfs:comment xml:lang="es">Esta propiedad relaciona las empresas con los productos o servicios (soluciones) de los que son consultores.</rdfs:comment>
        <rdfs:range rdf:resource="&v12;ProductOrService"/>
        <rdfs:domain rdf:resource="&org;Organization"/>
    </owl:ObjectProperty>
    


    <!-- http://minetur.linkeddata.es/def/ontologiaProductos#esFabricanteDe -->

    <owl:ObjectProperty rdf:about="http://minetur.linkeddata.es/def/ontologiaProductos#esFabricanteDe">
        <rdfs:label xml:lang="es">es fabricante de</rdfs:label>
        <rdfs:comment xml:lang="es">Esta propiedad relaciona las empresas con los productos o servicios (soluciones) de los que son fabricantes.</rdfs:comment>
        <rdfs:domain rdf:resource="&v12;BusinessEntity"/>
        <rdfs:subPropertyOf rdf:resource="&owl;topObjectProperty"/>
        <rdfs:range>
            <owl:Class>
                <owl:unionOf rdf:parseType="Collection">
                    <rdf:Description rdf:about="&v12;ProductOrService"/>
                    <rdf:Description rdf:about="&schema;Product"/>
                </owl:unionOf>
            </owl:Class>
        </rdfs:range>
    </owl:ObjectProperty>
    


    <!-- http://minetur.linkeddata.es/def/ontologiaProductos#esMayoristaDe -->

    <owl:ObjectProperty rdf:about="http://minetur.linkeddata.es/def/ontologiaProductos#esMayoristaDe">
        <rdfs:label xml:lang="es">es mayorista de</rdfs:label>
        <rdfs:comment xml:lang="es">Esta propiedad relaciona las empresas con los productos o servicios (soluciones) de los que son mayoristas.</rdfs:comment>
        <rdfs:range rdf:resource="&v12;ProductOrService"/>
        <rdfs:domain rdf:resource="&org;Organization"/>
    </owl:ObjectProperty>
    


    <!-- http://minetur.linkeddata.es/def/ontologiaProductos#tieneConsultor -->

    <owl:ObjectProperty rdf:about="http://minetur.linkeddata.es/def/ontologiaProductos#tieneConsultor">
        <rdfs:label xml:lang="es">tiene consultor</rdfs:label>
        <rdfs:comment xml:lang="es">Esta propiedad relaciona productos o servicios (soluciones) con las empresas que son consultoras de los mismos.</rdfs:comment>
        <owl:inverseOf rdf:resource="http://minetur.linkeddata.es/def/ontologiaProductos#esConsultorDe"/>
        <rdfs:domain rdf:resource="&v12;ProductOrService"/>
        <rdfs:range rdf:resource="&org;Organization"/>
    </owl:ObjectProperty>
    


    <!-- http://minetur.linkeddata.es/def/ontologiaProductos#tieneMayorista -->

    <owl:ObjectProperty rdf:about="http://minetur.linkeddata.es/def/ontologiaProductos#tieneMayorista">
        <rdfs:label xml:lang="es">tiene mayorista</rdfs:label>
        <rdfs:comment xml:lang="es">Esta propiedad relaciona productos o servicios (soluciones) con las empresas que son mayoristas de los mismos.</rdfs:comment>
        <owl:inverseOf rdf:resource="http://minetur.linkeddata.es/def/ontologiaProductos#esMayoristaDe"/>
        <rdfs:domain rdf:resource="&v12;ProductOrService"/>
        <rdfs:range rdf:resource="&org;Organization"/>
    </owl:ObjectProperty>
    


    <!-- http://purl.org/goodrelations/v1#hasManufacturer -->

    <owl:ObjectProperty rdf:about="&v12;hasManufacturer">
        <rdfs:label xml:lang="en">has manufacturer (0..1)</rdfs:label>
        <rdfs:comment xml:lang="en">This object property links a gr:ProductOrService to the gr:BusinessEntity that produces it. Mostly used with gr:ProductOrServiceModel.</rdfs:comment>
        <owl:inverseOf rdf:resource="http://minetur.linkeddata.es/def/ontologiaProductos#esFabricanteDe"/>
        <rdfs:isDefinedBy rdf:resource="http://purl.org/goodrelations/v1"/>
        <rdfs:range rdf:resource="&v12;BusinessEntity"/>
        <rdfs:domain>
            <owl:Class>
                <owl:unionOf rdf:parseType="Collection">
                    <rdf:Description rdf:about="&v12;ProductOrService"/>
                    <rdf:Description rdf:about="&schema;Product"/>
                </owl:unionOf>
            </owl:Class>
        </rdfs:domain>
    </owl:ObjectProperty>
    


    <!-- http://www.w3.org/ns/org#classification -->

    <owl:ObjectProperty rdf:about="&org;classification">
        <rdfs:label xml:lang="en">classification</rdfs:label>
        <rdfs:label xml:lang="es">pertenece a la clasificación</rdfs:label>
        <rdfs:label xml:lang="fr">classification</rdfs:label>
        <rdfs:label xml:lang="it">classificazione</rdfs:label>
        <rdfs:comment xml:lang="en">Indicates a classification for this Organization within some classification scheme. Extension vocabularies may wish to specialize this property to have a range corresponding to a specific `skos:ConceptScheme`. This property is under discussion and may be revised or removed - in many cases organizations are best categorized by defining a sub-class hierarchy in an extension vocabulary.</rdfs:comment>
        <rdfs:comment xml:lang="es">Ordenación jerárquica que se hace de una organización dentro de un esquema de clasificación. Es posible que algunos vocabularios especifiquen esta propiedad de forma que el rango se corresponda con un `skos:ConceptScheme` específico. La conveniencia de incluir esta propiedad se está debatiendo y puede que se revise o elimine (en muchos casos las organizaciones se clasifican mejor si se define una jerarquía de subclases en un vocabulario aparte)</rdfs:comment>
        <rdfs:comment xml:lang="fr">Indique une classification pour cette Organisation dans le cadre d&#39;un schéma de classification. Il est possible de spécialiser cette propriété en utilisant un vocabulaire spécialisé pour que le champ corresponde à un concept spécifique `skos:ConceptScheme`. Cette propriété est en discussion est pourrait être révisée ou supprimée - dans de nombreux cas, les organisations sont mieux catégorisées par une hiérarchie de sous-classe dans un vocabulaire externe.</rdfs:comment>
        <rdfs:comment xml:lang="it">Indica una classificazione per questa Organization all&#39;interno di un qualche schema di classificazione. Alcuni vocabolari potrebbero voler specializzare questa proprietà per avere un codominio corrispondente a uno specifico `skos:ConceptScheme`. Si noti che la presenza di questa proprietà è ancora in fase di discussione e potrebbe  essere revisionata o rimossa.</rdfs:comment>
        <rdfs:comment xml:lang="ja">ある分類表内のこの組織に対する分類を示します。
アプリケーションがorg:Organizationのサブクラスを組織的なカテゴリーを表わす手段として定義することも許容されることに注意してください。</rdfs:comment>
        <rdfs:range rdf:resource="&skos;Concept"/>
        <rdfs:isDefinedBy rdf:resource="http://www.w3.org/ns/org"/>
        <rdfs:domain rdf:resource="&org;Organization"/>
    </owl:ObjectProperty>
    


    <!-- http://xmlns.com/foaf/0.1/homepage -->

    <owl:ObjectProperty rdf:about="&foaf;homepage">
        <rdf:type rdf:resource="&owl;InverseFunctionalProperty"/>
        <rdfs:label>homepage</rdfs:label>
        <ns:term_status>stable</ns:term_status>
        <rdfs:comment>A homepage for some thing.</rdfs:comment>
        <rdfs:domain rdf:resource="&owl;Thing"/>
        <rdfs:subPropertyOf rdf:resource="&owl;topObjectProperty"/>
        <rdfs:isDefinedBy rdf:resource="http://xmlns.com/foaf/0.1/"/>
        <rdfs:range rdf:resource="&foaf;Document"/>
    </owl:ObjectProperty>
    


    <!-- http://xmlns.com/foaf/0.1/mbox -->

    <owl:ObjectProperty rdf:about="&foaf;mbox">
        <rdf:type rdf:resource="&owl;InverseFunctionalProperty"/>
        <rdfs:label>personal mailbox</rdfs:label>
        <rdfs:comment>A  personal mailbox, ie. an Internet mailbox associated with exactly one owner, the first owner of this mailbox. This is a &#39;static inverse functional property&#39;, in that  there is (across time and change) at most one individual that ever has any particular value for foaf:mbox.</rdfs:comment>
        <ns:term_status>stable</ns:term_status>
        <rdfs:range rdf:resource="&owl;Thing"/>
        <rdfs:isDefinedBy rdf:resource="http://xmlns.com/foaf/0.1/"/>
        <rdfs:domain rdf:resource="&foaf;Agent"/>
    </owl:ObjectProperty>
    


    <!-- 
    ///////////////////////////////////////////////////////////////////////////////////////
    //
    // Data properties
    //
    ///////////////////////////////////////////////////////////////////////////////////////
     -->

    


    <!-- http://purl.org/goodrelations/v1#category -->

    <owl:DatatypeProperty rdf:about="&v12;category">
        <rdfs:label xml:lang="en">category (0..*)</rdfs:label>
        <rdfs:comment xml:lang="en">The name of a category to which this gr:ProductOrService, gr:Offering, gr:BusinessEntity, or gr:Location belongs.
	
Note 1: For products, it is better to add an rdf:type statement referring to a GoodRelations-compliant ontology for vertical industries instead, but if you just have a short text label, gr:category is simpler.
Note 2: You can use greater signs or slashes to informally indicate a category hierarchy, e.g. &quot;restaurants/asian_restaurants&quot; or &quot;cables &gt; usb_cables&quot;
</rdfs:comment>
        <rdfs:isDefinedBy rdf:resource="http://purl.org/goodrelations/v1"/>
        <rdfs:range rdf:resource="&rdfs;Literal"/>
        <rdfs:domain rdf:resource="&owl;Thing"/>
    </owl:DatatypeProperty>
    


    <!-- http://purl.org/goodrelations/v1#description -->

    <owl:DatatypeProperty rdf:about="&v12;description">
        <rdfs:label xml:lang="en">description (0..1)</rdfs:label>
        <rdfs:comment xml:lang="en">A short textual description of the resource. 

This property is semantically equivalent to rdfs:comment and just meant as a handy shortcut for marking up data.</rdfs:comment>
        <rdfs:isDefinedBy rdf:resource="http://purl.org/goodrelations/v1"/>
        <rdfs:range rdf:resource="&rdfs;Literal"/>
        <rdfs:domain rdf:resource="&owl;Thing"/>
    </owl:DatatypeProperty>
    


    <!-- http://purl.org/goodrelations/v1#legalName -->

    <owl:DatatypeProperty rdf:about="&v12;legalName">
        <rdfs:label xml:lang="en">legal name (0..1)</rdfs:label>
        <rdfs:comment xml:lang="en">The legal name of the gr:BusinessEntity.</rdfs:comment>
        <rdfs:isDefinedBy rdf:resource="http://purl.org/goodrelations/v1"/>
        <rdfs:range rdf:resource="&rdfs;Literal"/>
        <rdfs:domain rdf:resource="&owl;Thing"/>
    </owl:DatatypeProperty>
    


    <!-- http://purl.org/goodrelations/v1#name -->

    <owl:DatatypeProperty rdf:about="&v12;name">
        <rdfs:label xml:lang="en">name (0..1)</rdfs:label>
        <rdfs:comment xml:lang="en">A short text describing the respective resource.

This property is semantically equivalent to dcterms:title and rdfs:label and just meant as a handy shortcut for marking up data.</rdfs:comment>
        <rdfs:isDefinedBy rdf:resource="http://purl.org/goodrelations/v1"/>
        <rdfs:range rdf:resource="&rdfs;Literal"/>
        <rdfs:domain rdf:resource="&owl;Thing"/>
    </owl:DatatypeProperty>
    


    <!-- http://www.loc.gov/mads/rdf/v1#phone -->

    <owl:DatatypeProperty rdf:about="&v1;phone">
        <rdfs:domain rdf:resource="&v1;Affiliation"/>
    </owl:DatatypeProperty>
    


    <!-- 
    ///////////////////////////////////////////////////////////////////////////////////////
    //
    // Classes
    //
    ///////////////////////////////////////////////////////////////////////////////////////
     -->

    


    <!-- http://purl.org/goodrelations/v1#BusinessEntity -->

    <owl:Class rdf:about="&v12;BusinessEntity"/>
    


    <!-- http://purl.org/goodrelations/v1#ProductOrService -->

    <owl:Class rdf:about="&v12;ProductOrService">
        <rdfs:label xml:lang="en">Product or service</rdfs:label>
        <rdfs:comment xml:lang="en">The superclass of all classes describing products or services types, either by nature or purpose. Examples for such subclasses are &quot;TV set&quot;, &quot;vacuum cleaner&quot;, etc. An instance of this class can be either an actual product or service (gr:Individual), a placeholder instance for unknown instances of a mass-produced commodity (gr:SomeItems), or a model / prototype specification (gr:ProductOrServiceModel). When in doubt, use gr:SomeItems.

Examples: 
a) MyCellphone123, i.e. my personal, tangible cell phone (gr:Individual)
b) Siemens1234, i.e. the Siemens cell phone make and model 1234 (gr:ProductOrServiceModel)
c) dummyCellPhone123 as a placeholder for actual instances of a certain kind of cell phones (gr:SomeItems)
	
Note: Your first choice for specializations of gr:ProductOrService should be http://www.productontology.org.

Compatibility with schema.org: This class is (approximately) equivalent to http://schema.org/Product.</rdfs:comment>
        <rdfs:isDefinedBy rdf:resource="http://purl.org/goodrelations/v1"/>
    </owl:Class>
    


    <!-- http://schema.org/Product -->

    <owl:Class rdf:about="&schema;Product"/>
    


    <!-- http://www.loc.gov/mads/rdf/v1#Affiliation -->

    <owl:Class rdf:about="&v1;Affiliation"/>
    


    <!-- http://www.w3.org/ns/org#FormalOrganization -->

    <owl:Class rdf:about="&org;FormalOrganization">
        <rdfs:subClassOf rdf:resource="&org;Organization"/>
    </owl:Class>
    


    <!-- http://www.w3.org/ns/org#Organization -->

    <owl:Class rdf:about="&org;Organization">
        <rdfs:label xml:lang="en">Organization</rdfs:label>
        <rdfs:label xml:lang="es">organización</rdfs:label>
        <rdfs:label xml:lang="fr">Organisation</rdfs:label>
        <rdfs:label xml:lang="it">Organizzazione</rdfs:label>
        <owl:equivalentClass rdf:resource="&foaf;Organization"/>
        <rdfs:subClassOf rdf:resource="&foaf;Agent"/>
        <rdfs:comment xml:lang="en">Represents a collection of people organized together into a community or other social, commercial or political structure. The group has some common purpose or reason for existence which goes beyond the set of people belonging to it and can act as an Agent. Organizations are often decomposable into hierarchical structures.  It is recommended that SKOS lexical labels should be used to label the Organization. In particular `skos:prefLabel` for the primary (possibly legally recognized name), `skos:altLabel` for alternative names (trading names, colloquial names) and `skos:notation` to denote a code from a code list. Alternative names: _Collective_ _Body_ _Org_ _Group_</rdfs:comment>
        <rdfs:comment xml:lang="es">Grupo de personas que se organiza en una comunidad u otro tipo de estructura social, comercial o política. Dicho grupo tiene un objetivo o motivo común para su existencia que va más allá del conjunto de personas que lo forman y que puede actuar como “agente”. A menudo las organizaciones se pueden agrupar en estructuras jerárquicas. Se recomienda el uso de etiquetas de SKOS para denominar a cada “organización”. En concreto, `skos:prefLabel` para la denominación principal o recomendada (aquella reconocida legalmente, siempre que sea posible), `skos:altLabel` para denominaciones alternativas (nombre comercial, sigla, denominación por la que se conoce a la organización coloquialmente) y `skos:notation` para referirse al código que identifique a la organización en una lista de códigos. Denominaciones alternativas: _colectivo_ _corporación_ _grupo_</rdfs:comment>
        <rdfs:comment xml:lang="fr">Représente un groupe de personnes organisées en communauté où tout autre forme de structure sociale, commerciale ou politique. Le groupe a un but commun ou une raison d&#39;être qui va au-delà de la somme des personnes qui en font partie et peut agir en tant que &quot;Agent&quot;. Les organisations sont souvent décomposables en structures hiérarchisées. Il est recommandé que des labels lexicaux SKOS soient utilisés pour nommer l&#39;Organisation. En particulier `skos:prefLabel` pour le nom principal (en général le nom légal), `skos:altLabel` pour les noms alternatifs (marques, sigles, appellations familières) et `skos:notation` pour indiquer un code provenant d&#39;une liste de code.</rdfs:comment>
        <rdfs:comment xml:lang="it">Rappresenta una collezione di persone organizzate all&#39;interno di una communità o di una qualche struttura sociale, commerciale o politica. Il gruppo condivide un obiettivo o una ragione d&#39;essere che va oltre gli stessi membri appartenenti al gruppo e  può agire come un Agent. Le organizzazioni si possono spesso suddividere in strutture gerarchiche. Si raccomanda di usare le label per l&#39;Organization mediante le proprietà di SKOS. In particolare, `skos:prefLabel` per il nome principale (possibilmente un nome legalmente riconosciuto)”, `skos:altLabel` come nome alternativo (denominazione commerciale, denominazione colloquiale) e `skos:notation` per indicare un codice di una lista di codici.</rdfs:comment>
        <rdfs:comment xml:lang="ja">コミュニティー、その他の社会、商業、政治的な構造に共に編入された人々の集合を表わします。グループには、そこに属する人々を超えた、存在に対するある共通の目的や理由があり、エージェント（代理）を務めることができます。組織は、多くの場合、階層構造に分割できます。</rdfs:comment>
        <rdfs:isDefinedBy rdf:resource="http://www.w3.org/ns/org"/>
    </owl:Class>
    


    <!-- http://www.w3.org/ns/org#OrganizationalCollaboration -->

    <owl:Class rdf:about="&org;OrganizationalCollaboration">
        <rdfs:subClassOf rdf:resource="&org;Organization"/>
    </owl:Class>
    


    <!-- http://www.w3.org/ns/org#OrganizationalUnit -->

    <owl:Class rdf:about="&org;OrganizationalUnit">
        <rdfs:subClassOf rdf:resource="&org;Organization"/>
    </owl:Class>
    


    <!-- http://xmlns.com/foaf/0.1/Agent -->

    <owl:Class rdf:about="&foaf;Agent">
        <rdfs:label>Agent</rdfs:label>
        <ns:term_status>stable</ns:term_status>
        <rdfs:comment>An agent (eg. person, group, software or physical artifact).</rdfs:comment>
    </owl:Class>
    


    <!-- http://xmlns.com/foaf/0.1/Document -->

    <owl:Class rdf:about="&foaf;Document">
        <rdfs:label>Document</rdfs:label>
        <owl:disjointWith rdf:resource="&foaf;Organization"/>
        <ns:term_status>stable</ns:term_status>
        <rdfs:comment>A document.</rdfs:comment>
        <rdfs:isDefinedBy rdf:resource="http://xmlns.com/foaf/0.1/"/>
    </owl:Class>
    


    <!-- http://xmlns.com/foaf/0.1/Group -->

    <owl:Class rdf:about="&foaf;Group">
        <rdfs:subClassOf rdf:resource="&foaf;Agent"/>
    </owl:Class>
    


    <!-- http://xmlns.com/foaf/0.1/Organization -->

    <owl:Class rdf:about="&foaf;Organization">
        <rdfs:label>Organization</rdfs:label>
        <rdfs:subClassOf rdf:resource="&foaf;Agent"/>
        <owl:disjointWith rdf:resource="&foaf;Person"/>
        <ns:term_status>stable</ns:term_status>
        <rdfs:comment>An organization.</rdfs:comment>
        <rdfs:isDefinedBy rdf:resource="http://xmlns.com/foaf/0.1/"/>
    </owl:Class>
    


    <!-- http://xmlns.com/foaf/0.1/Person -->

    <owl:Class rdf:about="&foaf;Person">
        <rdfs:subClassOf rdf:resource="&foaf;Agent"/>
    </owl:Class>
    <rdf:Description>
        <v12:description>VGhlIFNldmVuIE5vYWhpZGUgTGF3cw0KMS4gQmVsaWVmIGluIEctZA0KMi4gUmVzcGVjdCBHLWQgYW5kIHByYWlzZSBoaW0NCjMuIFJlc3BlY3QgaHVtYW4gbGlmZQ0KNC4gUmVzcGVjdCB0aGUgZmFtaWx5DQo1LiBSZXNwZWN0IGh1bWFuIGJlaW5ncw0KNi4gSGF2ZSBhIGp1ZGljaWFsIHN5c3RlbQ0KNy4gUmVzcGVjdCBhbGwgY3JlYXR1cmVz</v12:description>
        <v12:category>42</v12:category>
    </rdf:Description>
</rdf:RDF>



<!-- Generated by the OWL API (version 3.2.3.1824) http://owlapi.sourceforge.net -->

